nat_seqs.v
@@ -122,7 +122,7 @@ Qed.
 Require Import Relations.
 Require vec.
 
-Lemma filtered_sort (T: Set) (R: relation T) (P: preorder T R) (p: T -> T -> bool) (pc: forall x y, p y x = true -> ~ R y x) (l: list T): vec.sorted R l ->
+Lemma filtered_sort (T: Set) (R: relation T) (P: preorder T R) (p: T -> T -> bool) (pc: forall x y, p y x = true -> ~ R y x) (l: list T): vec.sorted R (vec.from_list l) ->
   elemsR le (map (fun x => length (filter (p (fst x)) (snd x))) (splits l)) (nats 0 (length l)).
 Proof with auto.
   induction l.
