ne_tree.v
@@ -41,7 +41,7 @@ Section contents.
 
   Definition T_rec (P: T -> Set) (Pleaf: forall n, P (Leaf n)) (Pone: forall t, P t -> P (Node (ne_list.one t))) (Pcons: forall t l, P t -> P (Node l) -> P (Node (ne_list.cons t l))): forall t, P t := T_rect P Pleaf Pone Pcons.
 
-  Definition alt_ind (P: T -> Prop) (Pleaf: forall n, P (Leaf n)) (Pnode: forall l:ne_list.L T, (forall t, List.In t l -> P t) -> P (Node l)) (t: T): P t.
+  Definition alt_ind (P: T -> Prop) (Pleaf: forall n, P (Leaf n)) (Pnode: forall l:ne_list.L T, (forall t, List.In t (ne_list.to_plain l) -> P t) -> P (Node l)) (t: T): P t.
   Proof with auto.
     revert P Pleaf Pnode t.
     intros P Hbase Hrcd.
@@ -118,7 +118,7 @@ Section contents.
     | InTail t l: InL e l -> InL e (ne_list.cons t l).
 
   Lemma InL_map_inv (Q: Set) (e: E) (f: Q -> T) (l: ne_list.L Q):
-    InL e (ne_list.map f l) -> exists e', In e (f e') /\ List.In e' l.
+    InL e (ne_list.map f l) -> exists e', In e (f e') /\ List.In e' (ne_list.to_plain l).
   Proof with auto.
     induction l.
       simpl.
