sums_and_averages.v
@@ -1,4 +1,3 @@
-
 Set Implicit Arguments.
 
 Require Import
@@ -679,4 +678,4 @@ Proof. unfold Ravg. simpl. intros. field. Qed.
 
 Require ne_tree.
 
-Definition TRavg: ne_tree.T R -> R := ne_tree.fold (@id R) Ravg.
+Definition TRavg: ne_tree.T R -> R := ne_tree.fold (@id R) (fun l => Ravg (ne_list.to_plain l)).
